GraphMSO/Automata.lean
@@ -1,5 +1,7 @@
 import GraphMSO.Automata.term
 import GraphMSO.Automata.automaton
 import GraphMSO.Automata.binTree
+import GraphMSO.Automata.atomic
 import GraphMSO.Automata.projection
+import GraphMSO.Automata.compile
 import GraphMSO.Automata.emptiness
